Changed the programs' code to be shorter

Loop/Basic.lean
@@ -76,62 +76,57 @@ theorem get_is_loop_computable_cleanly (i : Fin n) : loop_computable_cleanly (fu
   simp [init_state, highest_var, this, p, execution_from_state,
     loop_inc_adds_value, value_at_cons_succ, value_at, Mathlib.Vector.get_eq_get]
 
-theorem comp_is_loop_computable_cleanly (g : Fin n → VectNat m → Nat) :
-      loop_computable_cleanly f
-    → (∀ i, loop_computable_cleanly (g i))
-    → loop_computable_cleanly fun a => f (Mathlib.Vector.ofFn fun i => g i a) := by
-  sorry
+-- theorem comp_is_loop_computable_cleanly (g : Fin n → VectNat m → Nat) :
+--       loop_computable_cleanly f
+--     → (∀ i, loop_computable_cleanly (g i))
+--     → loop_computable_cleanly fun a => f (Mathlib.Vector.ofFn fun i => g i a) := by
+--   sorry
 
 section prec_is_loop_computable_cleanly_proof
 
-variable {n : Nat} {f : VectNat n → Nat} {g : VectNat (n + 2) → Nat}
+variable {n : Nat} {f : VectNat n → Nat} {g : VectNat (n + 2) → Nat} (f_h : cleanly_computes p_f f) (g_h : cleanly_computes p_g g)
 
 -- Part I: construction of the program
 
 def offset (_ : cleanly_computes p_f f) (_ : cleanly_computes p_g g) : Nat :=  max (n + 2) (max (highest_var p_f) (highest_var p_g))
 
--- Step 1: compute f of the last n inputs and store the result in the
--- 'result' variable
-def prec_program_1 (f_h : cleanly_computes p_f f) (g_h : cleanly_computes p_g g) : Program :=
+-- Step 1: compute f of the last n inputs
+def prec_program_1 : Program :=
   let offset := offset f_h g_h
-  let p_1_1 := store_X_1_to_X_succ_n (offset + 2) n
+  let p_1_1 := store_X_1_to_X_succ_n (offset + 1) n
   let p_1_2 := clear_X_j_to_X_n_plus_j 1 n
   let p_1_3 := match (generalizing := false) n with
     | 0 => p_f
-    | n + 1 => setup_X_j_to_X_n_plus_j (offset + 2) 1 n ++ p_f
-  let p_1_4 := X (offset + 1) += X 0
-  let p_1_5 := CLEAR X 0
-  p_1_1 ++ p_1_2 ++ p_1_3 ++ p_1_4 ++ p_1_5
+    | n + 1 => setup_X_j_to_X_n_plus_j (offset + 1) 1 n ++ p_f
+  p_1_1 ++ p_1_2 ++ p_1_3
 
 -- Step 2: compute g counter number of times, for each recursive step
-def prec_program_2 (f_h : cleanly_computes p_f f) (g_h : cleanly_computes p_g g) : Program :=
+def prec_program_2 : Program :=
   let offset := offset f_h g_h
-  let p_2_1 := X 2 += X (offset + 1)
-  let p_2_2 := match n with
-    | 0 => p_g
-    | n + 1 => setup_X_j_to_X_n_plus_j (offset + 2) 3 n ++ p_g
-  let p_2_3 := CLEAR X (offset + 1) ++ X (offset + 1) += X 0
-  let p_2_4 := CLEAR X 0
+  let p_2_1 := X 2 += X 0
+  let p_2_2 := CLEAR X 0
+  let p_2_3 := p_g
+  let p_2_4 := CLEAR X 2
   let p_2_5 := INC X 1
   let loop_inner := p_2_1 ++ p_2_2 ++ p_2_3 ++ p_2_4 ++ p_2_5
-  let p_loop := LOOP X (offset + 2) DO loop_inner END
-  match n with
+  let p_loop := LOOP X (offset + 1) DO loop_inner END
+  match (generalizing := false) n with
     | 0 => p_loop
-    | n + 1 => clear_X_j_to_X_n_plus_j 1 n ++ p_loop
+    | n + 1 => clear_X_j_to_X_n_plus_j 1 n ++ setup_X_j_to_X_n_plus_j (offset + 1) 3 n ++ p_loop
 
 -- Step 3: Clean up
-def prec_program_3 (f_h : cleanly_computes p_f f) (g_h : cleanly_computes p_g g) : Program :=
+def prec_program_3 : Program :=
   let offset := offset f_h g_h
-  let p_3_1 := X 0 += X (offset + 1)
-  let p_3_2 := clear_X_j_to_X_n_plus_j 1 (n + 1)
-  let p_3_3 := match n with
-    | 0 => X 1 += X (offset + 2)
-    | n + 1 => setup_X_j_to_X_n_plus_j (offset + 2) 2 n
-  let p_3_4 := CLEAR X (offset + 1)
-  let p_3_5 := clear_Z_0_to_Z_n (offset + 2) n
-  p_3_1 ++ p_3_2 ++ p_3_3 ++ p_3_4 ++ p_3_5
+  let p_3_1 := match (generalizing := false) n with
+    | 0 => CLEAR X 1
+    | n + 1 => CLEAR X 1 ++ clear_X_j_to_X_n_plus_j 3 n
+  let p_3_2 := match (generalizing := false) n with
+    | 0 => X 1 += X (offset + 1)
+    | n + 1 => setup_X_j_to_X_n_plus_j (offset + 1) 2 n
+  let p_3_3 := clear_Z_0_to_Z_n (offset + 1) n
+  p_3_1 ++ p_3_2 ++ p_3_3
 
-def prec_program (f_h : cleanly_computes p_f f) (g_h : cleanly_computes p_g g) : Program :=
+def prec_program : Program :=
   let p_1 := prec_program_1 f_h g_h
   let p_2 := prec_program_2 f_h g_h
   let p_3 := prec_program_3 f_h g_h
@@ -139,8 +134,7 @@ def prec_program (f_h : cleanly_computes p_f f) (g_h : cleanly_computes p_g g) :
 
 -- Part II: calculate the highest variable of the program
 
-theorem prec_program_1_highest_var (f_h : cleanly_computes p_f f) (g_h : cleanly_computes p_g g) :
-    highest_var (prec_program_1 f_h g_h) = offset f_h g_h + 2 + n := by
+theorem prec_program_1_highest_var : highest_var (prec_program_1 f_h g_h) = offset f_h g_h + 1 + n := by
   simp [prec_program_1]
   repeat rewrite [highest_var_concat]
   rewrite [highest_var_store, highest_var_clear]
@@ -149,122 +143,115 @@ theorem prec_program_1_highest_var (f_h : cleanly_computes p_f f) (g_h : cleanly
   case zero =>
     simp_arith
     have : highest_var p_f ≤ offset f_h g_h := by simp [offset]
-    exact Nat.le_trans this (Nat.le_add_right _ 2)
+    exact Nat.le_trans this (Nat.le_add_right _ 1)
   case succ n =>
     rewrite [highest_var_concat, highest_var_setup]
-    have : max (n + 1 + 1) (offset f_h g_h + 2 + (n + 1)) = offset f_h g_h + 2 + (n + 1) := by simp_arith
+    have : max (n + 1 + 1) (offset f_h g_h + 1 + (n + 1)) = offset f_h g_h + 1 + (n + 1) := by simp_arith
     rewrite [this]
-    have : max (n + 1) (offset f_h g_h + 2 + n + 1) = offset f_h g_h + 2 + n + 1 := by simp_arith
+    have : max (n + 1) (offset f_h g_h + 1 + n + 1) = offset f_h g_h + 1 + n + 1 := by simp_arith
     rewrite [this]
-    have : max (offset f_h g_h + 2 + n + 1) (highest_var p_f) = offset f_h g_h + 2 + n + 1 := by
+    have : max (offset f_h g_h + 1 + n + 1) (highest_var p_f) = offset f_h g_h + 1 + n + 1 := by
       simp_arith
       have : highest_var p_f ≤ offset f_h g_h := by simp [offset]
-      exact Nat.le_trans this (Nat.le_add_right _ (n + 3))
+      exact Nat.le_trans this (Nat.le_add_right _ (n + 2))
     rewrite [this]
-    have : (max (offset f_h g_h + 2 + (n + 1)) (offset f_h g_h + 2 + n + 1)) = offset f_h g_h + 2 + n + 1 := by
+    have : (max (offset f_h g_h + 1 + (n + 1)) (offset f_h g_h + 1 + n + 1)) = offset f_h g_h + 1 + n + 1 := by
       repeat rewrite [←Nat.add_assoc]
       exact Nat.max_self _
     rewrite [this]
     simp_arith
 
-theorem prec_program_2_highest_var (f_h : cleanly_computes p_f f) (g_h : cleanly_computes p_g g) :
-    highest_var (prec_program_2 f_h g_h) = offset f_h g_h + 2 + n := by
+theorem prec_program_2_highest_var : highest_var (prec_program_2 f_h g_h) = offset f_h g_h + 1 + n := by
+
   simp [prec_program_2]
   cases n
   case zero =>
-    simp [highest_var, ]
+    simp [highest_var]
+    constructor
+    simp [offset]
     have : highest_var p_g ≤ offset f_h g_h := by simp [offset]
-    exact Nat.le_trans this (Nat.le_add_right _ 2)
+    exact Nat.le_trans this (Nat.le_add_right _ 1)
   case succ n =>
-    simp [highest_var, highest_var_clear]
-    rewrite [highest_var_setup]
-    have : max (n + 3) (offset f_h g_h + 2 + n + 1) = offset f_h g_h + 2 + n + 1 := by simp_arith
+    simp [highest_var, highest_var_clear, highest_var_setup]
+    have : max (n + 3) (offset f_h g_h + 1 + n + 1) = offset f_h g_h + 1 + n + 1 := by simp_arith [offset]
     rewrite [this]
-    have : max (offset f_h g_h + 2 + n + 1) (highest_var p_g) = offset f_h g_h + 2 + n + 1 := by
-      simp_arith
-      have : highest_var p_g ≤ offset f_h g_h := by simp [offset]
-      exact Nat.le_trans this (Nat.le_add_right _ (n + 3))
+    have : max (offset f_h g_h + 1) (max 2 (highest_var p_g)) = offset f_h g_h + 1 := by
+      have h1 : offset f_h g_h + 1 ≥ 2 := by simp [offset]
+      have h2 : offset f_h g_h + 1 ≥ highest_var p_g := by exact calc
+        highest_var p_g ≤ offset f_h g_h := by simp [offset]
+                      _ ≤ offset f_h g_h + 1 := by simp_arith
+      have := Nat.max_le_of_le_of_le h1 h2
+      rewrite [Nat.max_comm]
+      exact Nat.max_eq_right this
     rewrite [this]
-    have : max (max (offset f_h g_h + 1) 2) (offset f_h g_h + 2 + n + 1) = offset f_h g_h + 2 + n + 1 := by
-      have : max (offset f_h g_h + 1) 2 ≤ offset f_h g_h + 2 + n + 1 := by
-        simp_arith
-        rw [Nat.add_assoc]
-        exact Nat.le_add_right _ _
-      rewrite [Nat.max_def]
-      simp [this]
-    rewrite [this]
-    simp_arith
+    have : max (offset f_h g_h + 1 + n + 1) (offset f_h g_h + 1) = offset f_h g_h + 1 + n + 1 := by
+      simp
+      -- offset f_h g_h ≤ offset f_h g_h + 1 + n
+      exact calc
+        offset f_h g_h ≤ offset f_h g_h := by exact Nat.le_refl (offset f_h g_h)
+                     _ ≤ offset f_h g_h + (1 + n) := by simp
+                     _ = offset f_h g_h + 1 + n := by rw [Nat.add_assoc]
+    rw [this, Nat.add_assoc]
 
-theorem prec_program_3_highest_var (f_h : cleanly_computes p_f f) (g_h : cleanly_computes p_g g) :
-    highest_var (prec_program_3 f_h g_h) = offset f_h g_h + 2 + n := by
+theorem prec_program_3_highest_var : highest_var (prec_program_3 f_h g_h) = offset f_h g_h + 1 + n := by
   simp [prec_program_3]
-  repeat rewrite [highest_var_concat]
-  rewrite [highest_var_clear, highest_var_clear_Z]
   cases n
   case zero =>
-    simp [highest_var]
+    simp [inc_X_i_X_j, highest_var]
   case succ n =>
-    simp [highest_var_setup, highest_var]
-    repeat constructor
-    · simp_arith
-    · have : offset f_h g_h + 2 + (n + 1) = n + 1 + 1 + 1 + offset f_h g_h := by simp_arith
-      rewrite [this]
-      simp
-    constructor
-    · have : offset f_h g_h + 2 + (n + 1) = n + 1 + 1 + offset f_h g_h + 1 := by simp_arith
-      rewrite [this]
-      simp_arith
-    · repeat rw [Nat.add_assoc]
+    simp [highest_var]
+    rewrite [highest_var_clear, highest_var_clear_Z, highest_var_setup]
+    simp_arith [offset]
 
-theorem prec_program_highest_var (f_h : cleanly_computes p_f f) (g_h : cleanly_computes p_g g) :
-    highest_var (prec_program f_h g_h) = offset f_h g_h + 2 + n := by
+theorem prec_program_highest_var : highest_var (prec_program f_h g_h) = offset f_h g_h + 1 + n := by
   simp [prec_program]
   repeat rewrite [highest_var_concat]
   rewrite [prec_program_1_highest_var, prec_program_2_highest_var, prec_program_3_highest_var]
   repeat rw [Nat.max_self]
 
-theorem execution_from_state_prec_program_1_1 (f_h : cleanly_computes p_f f) (g_h : cleanly_computes p_g g) (v : VectNat (n + 1)) :
-    execution_from_state (0 :: (v.toList ++ 0 :: (List.zeros (offset f_h g_h - (n + 2)) ++ 0 :: 0 :: List.zeros n))) (store_X_1_to_X_succ_n (offset f_h g_h + 2) n)
-      = 0 :: v.toList ++ 0 :: List.zeros (offset f_h g_h - (n + 2)) ++ 0 :: v.toList := by
+theorem execution_from_state_prec_program_1_1 (v : VectNat (n + 1)) :
+    execution_from_state (0 :: (v.toList ++ 0 :: (List.zeros (offset f_h g_h - (n + 2)) ++  0 :: List.zeros n))) (store_X_1_to_X_succ_n (offset f_h g_h + 1) n)
+      = 0 :: v.toList ++ 0 :: List.zeros (offset f_h g_h - (n + 2)) ++ v.toList := by
   let c :=  offset f_h g_h - (n + 2)
   have : offset f_h g_h - (n + 2) = c := rfl
   rewrite [this]
-  have : offset f_h g_h + 2 = c + n + 4 := by
+  have : offset f_h g_h + 1 = c + n + 3 := by
     simp [c]
     rewrite [Nat.add_assoc]
     have : n + 2 ≤ offset f_h g_h := Nat.le_max_left _ _
     rw [Nat.sub_add_cancel this]
   rewrite [this]
-  let w := 0 :: List.zeros c ++ [0]
-  have w_l : w.length = c + 2:= by simp [w, c]
-
-  have := lemma_store (c + 2) n ⟨w, w_l⟩ v
-  simp_arith [w] at this
-  simp
+  let w := 0 :: List.zeros c
+  have w_l : w.length = c + 1 := by simp [w, c]
+  have := lemma_store (c + 1) n ⟨w, w_l⟩ v
+  dsimp [w] at this
+  rewrite [zeros_succ] at this
+  simp_arith at this
   rewrite [Nat.add_comm c n]
+  simp
   exact this
 
-theorem execution_from_state_prec_program_1_2 (f_h : cleanly_computes p_f f) (g_h : cleanly_computes p_g g) (v : VectNat (n + 1)) :
-    execution_from_state (0 :: v.toList ++ 0 :: List.zeros (offset f_h g_h - (n + 2)) ++ 0 :: v.toList) (clear_X_j_to_X_n_plus_j 1 n)
-      = 0 :: List.zeros (n + 1) ++ 0 :: List.zeros (offset f_h g_h - (n + 2)) ++ 0 :: v.toList := by
+theorem execution_from_state_prec_program_1_2 (v : VectNat (n + 1)) :
+    execution_from_state (0 :: v.toList ++ 0 :: List.zeros (offset f_h g_h - (n + 2)) ++ v.toList) (clear_X_j_to_X_n_plus_j 1 n)
+      = 0 :: List.zeros (n + 1) ++ 0 :: List.zeros (offset f_h g_h - (n + 2)) ++ v.toList := by
   have : highest_var (clear_X_j_to_X_n_plus_j 1 n) ≤ n + 1 := by
     have : highest_var (clear_X_j_to_X_n_plus_j 1 n) = n + 1 := highest_var_clear
     rewrite [this]
     exact Nat.le_refl _
-  have := @execution_from_state_gt_highest_append (clear_X_j_to_X_n_plus_j 1 n) (0 :: List.zeros (offset f_h g_h - (n + 2)) ++ 0 :: Mathlib.Vector.toList v)
+  have := @execution_from_state_gt_highest_append (clear_X_j_to_X_n_plus_j 1 n) (0 :: List.zeros (offset f_h g_h - (n + 2)) ++ Mathlib.Vector.toList v)
     (n + 1) ⟨0 :: v.toList, by simp⟩ this
   simp at this
   simp
   rw [this, clear_X_lemma]
   simp
 
-theorem execution_from_state_prec_program_1_3 (f_h : cleanly_computes p_f f) (g_h : cleanly_computes p_g g) (v : VectNat (n + 1)) :
-    execution_from_state (0 :: List.zeros (n + 1) ++ 0 :: List.zeros (offset f_h g_h - (n + 2)) ++ 0 :: v.toList) (match n with | 0 => p_f | n + 1 => setup_X_j_to_X_n_plus_j (offset f_h g_h + 2) 1 n ++ p_f)
-      = f v.tail :: v.tail.toList ++ 0 :: 0 :: List.zeros (offset f_h g_h - (n + 2)) ++ 0 :: v.toList := by
+theorem execution_from_state_prec_program_1_3 (v : VectNat (n + 1)) :
+    execution_from_state (0 :: List.zeros (n + 1) ++ 0 :: List.zeros (offset f_h g_h - (n + 2)) ++ v.toList) (match n with | 0 => p_f | n + 1 => setup_X_j_to_X_n_plus_j (offset f_h g_h + 1) 1 n ++ p_f)
+      = f v.tail :: v.tail.toList ++ 0 :: 0 :: List.zeros (offset f_h g_h - (n + 2)) ++ v.toList := by
   cases n
   case zero =>
     simp
-    have : 0 :: 0 :: 0 :: (List.zeros (offset f_h g_h - 2) ++ [0, v.head]) = 0 :: (0 :: 0 :: List.zeros (offset f_h g_h - 2)) ++ [0, v.head] := by simp
+    have : 0 :: 0 :: 0 :: (List.zeros (offset f_h g_h - 2) ++ [v.head]) = 0 :: (0 :: 0 :: List.zeros (offset f_h g_h - 2)) ++ [v.head] := by simp
     rewrite [this]
     have z_h : 0 :: 0 :: List.zeros (offset f_h g_h - 2) = List.zeros (offset f_h g_h) := by
       repeat rewrite [←zeros_succ]
@@ -273,12 +260,12 @@ theorem execution_from_state_prec_program_1_3 (f_h : cleanly_computes p_f f) (g_
         rw [Nat.sub_add_cancel this]
       rw [this]
     rewrite [z_h]
-    have := @cleanly_computable_append_zeros_append_xs 0 p_f f (offset f_h g_h) f_h (0 :: v.toList) Mathlib.Vector.nil (by simp [offset])
+    have := @cleanly_computable_append_zeros_append_xs 0 p_f f (offset f_h g_h) f_h v.toList Mathlib.Vector.nil (by simp [offset])
     simp [init_state] at this
     simp
     rewrite [this]
     simp
-    have : 0 :: 0 :: (List.zeros (offset f_h g_h - 2) ++ [0, v.head]) = List.zeros (offset f_h g_h) ++ [0, v.head] := by
+    have : 0 :: 0 :: (List.zeros (offset f_h g_h - 2) ++ [v.head]) = List.zeros (offset f_h g_h) ++ [v.head] := by
       repeat rewrite [←List.cons_append]
       rw [z_h]
     rw [this]
@@ -287,42 +274,52 @@ theorem execution_from_state_prec_program_1_3 (f_h : cleanly_computes p_f f) (g_
     simp at xs_l
     rewrite [List.zeros_concat]
     simp [concat_is_seq_execution, execution_from_state, Mathlib.Vector.tail]
-    have list_zeros : 0 :: 0 :: List.zeros (offset f_h g_h - (n + 1 + 2)) ++ [0] = List.zeros (offset f_h g_h - n) := by
+    have list_zeros : 0 :: 0 :: List.zeros (offset f_h g_h - (n + 1 + 2)) = List.zeros (offset f_h g_h - (n + 1)) := by
       repeat rewrite [←zeros_succ]
-      rewrite [←List.zeros_concat]
-      -- There's definitely redundant code somewhere, but it works
-      have : n + 1 + 2 = n + 3 := by rw [Nat.add_assoc]
-      simp_arith [this]
-      rewrite [Nat.sub_add_eq]
-      suffices h : offset f_h g_h - n ≥ 3 from by rw [Nat.sub_add_cancel h]
-      suffices h : offset f_h g_h ≥ 3 + n from by
-        have := Nat.sub_le_sub_right h n
-        rewrite [Nat.add_sub_cancel 3 n] at this
+      suffices h : offset f_h g_h - (n + 1 + 2) + 1 + 1 = offset f_h g_h - (n + 1) from by rw [h]
+      rewrite [Nat.add_assoc, Nat.sub_add_eq]
+      have : 1 + 1 = 2 := rfl
+      rewrite [this]
+      suffices h : offset f_h g_h - (n + 1) ≥ 2 from Nat.sub_add_cancel h
+      suffices h : offset f_h g_h ≥ 2 + (n + 1) from by
+        have := Nat.sub_le_sub_right h (n + 1)
+        rewrite [Nat.add_sub_cancel 2 (n + 1)] at this
         assumption
-      rewrite [Nat.add_comm 3 n]
+      rewrite [Nat.add_comm 2 (n + 1)]
       exact by calc
         offset f_h g_h ≥ n + 1 + 2 := by dsimp [offset]; exact Nat.le_max_left _ _
                      _ = n + 3 := by rw [Nat.add_assoc]
-    have : List.zeros (n + 1) ++ 0 :: 0 :: (List.zeros (offset f_h g_h - (n + 1 + 2)) ++ 0 :: x :: xs)
-      = List.zeros (n + 1) ++ List.zeros (offset f_h g_h - n) ++ x :: xs := by exact calc
-            List.zeros (n + 1) ++ 0 :: 0 :: (List.zeros (offset f_h g_h - (n + 1 + 2)) ++ 0 :: x :: xs)
-                = List.zeros (n + 1) ++ (0 :: 0 :: List.zeros (offset f_h g_h - (n + 1 + 2)) ++ [0]) ++ x :: xs := by simp
-              _ = List.zeros (n + 1) ++ List.zeros (offset f_h g_h - n) ++ x :: xs := by rw [list_zeros]
+    have : List.zeros (n + 1) ++ 0 :: 0 :: (List.zeros (offset f_h g_h - (n + 1 + 2)) ++ x :: xs)
+      = List.zeros (n + 1) ++ List.zeros (offset f_h g_h - (n + 1)) ++ x :: xs := by exact calc
+            List.zeros (n + 1) ++ 0 :: 0 :: (List.zeros (offset f_h g_h - (n + 1 + 2)) ++x :: xs)
+                = List.zeros (n + 1) ++ (0 :: 0 :: List.zeros (offset f_h g_h - (n + 1 + 2))) ++ x :: xs := by simp
+              _ = List.zeros (n + 1) ++ List.zeros (offset f_h g_h - (n + 1)) ++ x :: xs := by rw [list_zeros]
     rewrite [this]
-    have : (xs ++ 0 :: 0 :: (List.zeros (offset f_h g_h - (n + 1 + 2)) ++ 0 :: x :: xs))
-      = xs ++ List.zeros (offset f_h g_h - n) ++ x :: xs := by exact calc
-            xs ++ 0 :: 0 :: (List.zeros (offset f_h g_h - (n + 1 + 2)) ++ 0 :: x :: xs)
-                = xs ++ (0 :: 0 :: List.zeros (offset f_h g_h - (n + 1 + 2)) ++ [0]) ++ x :: xs := by simp
-              _ = xs ++ List.zeros (offset f_h g_h - n) ++ x :: xs := by rw [list_zeros]
+    have : (xs ++ 0 :: 0 :: (List.zeros (offset f_h g_h - (n + 1 + 2)) ++ x :: xs))
+      = xs ++ List.zeros (offset f_h g_h - (n + 1)) ++ x :: xs := by exact calc
+            xs ++ 0 :: 0 :: (List.zeros (offset f_h g_h - (n + 1 + 2)) ++ x :: xs)
+                = xs ++ (0 :: 0 :: List.zeros (offset f_h g_h - (n + 1 + 2))) ++ x :: xs := by simp
+              _ = xs ++ List.zeros (offset f_h g_h - (n + 1)) ++ x :: xs := by rw [list_zeros]
     rewrite [this]
     --
-    have : List.zeros (n + 1) ++ List.zeros (offset f_h g_h - n) ++ x :: xs
-      = List.zeros (n + 1) ++ (List.zeros (offset f_h g_h - n) ++ [x]) ++ xs := by rewrite [List.append_assoc] ; simp
+    have : List.zeros (n + 1) ++ List.zeros (offset f_h g_h - (n + 1)) ++ x :: xs
+      = List.zeros (n + 1) ++ (List.zeros (offset f_h g_h - (n + 1)) ++ [x]) ++ xs := by rewrite [List.append_assoc] ; simp
     rewrite [this]
-    have : (List.zeros (offset f_h g_h - n) ++ [x]).length = offset f_h g_h - n + 1 := by simp
-    have := lemma_setup (offset f_h g_h - n + 1) n ⟨List.zeros (offset f_h g_h - n) ++ [x], this⟩ ⟨xs, xs_l⟩
+    have : (List.zeros (offset f_h g_h - (n + 1)) ++ [x]).length = offset f_h g_h - n := by
+      simp
+      rewrite [Nat.sub_add_eq]
+      suffices h : offset f_h g_h - n ≥ 1 from Nat.sub_add_cancel h
+      exact calc
+        offset f_h g_h - n ≥ (n + 1 + 2) - n := by
+          dsimp [offset]
+          exact Nat.sub_le_sub_right (Nat.le_max_left (n + 1 + 2) (max (highest_var p_f) (highest_var p_g))) n
+        _ ≥ 1 := by
+          rewrite [Nat.add_comm, Nat.add_comm n, ←Nat.add_assoc, Nat.add_sub_cancel]
+          simp_arith
+    have := lemma_setup (offset f_h g_h - n) n ⟨List.zeros (offset f_h g_h - (n + 1)) ++ [x], this⟩ ⟨xs, xs_l⟩
     dsimp [Mathlib.Vector.toList] at this
-    have lemm_eq : n + (offset f_h g_h - n + 1) + 1 = offset f_h g_h + 2 := by
+
+    have lemm_eq : n + (offset f_h g_h - n) + 1 = offset f_h g_h + 1 := by
       simp_arith
       rewrite [Nat.add_comm]
       suffices h : n ≤ offset f_h g_h from by exact Nat.sub_add_cancel h
@@ -330,64 +327,40 @@ theorem execution_from_state_prec_program_1_3 (f_h : cleanly_computes p_f f) (g_
         n ≤ n + 1 + 2 := by simp_arith
         _  ≤ offset f_h g_h := by dsimp [offset]; exact Nat.le_max_left _ _
     rewrite [lemm_eq] at this
-
     rewrite [this]
     rewrite [←List.cons_append, ←List.cons_append]
     rewrite [←List.append_assoc]
-    have : offset f_h g_h - n ≥ highest_var p_f - (n + 1) := by
-      have : offset f_h g_h ≥ highest_var p_f := by simp [offset]
-      have : offset f_h g_h - n ≥ highest_var p_f - n := Nat.sub_le_sub_right this n
-      suffices h : highest_var p_f - (n + 1) ≤ highest_var p_f - n from Nat.le_trans h this
-      suffices h : n + 1 ≥ n from Nat.sub_le_sub_left h _
-      simp_arith
+    have : offset f_h g_h - (n + 1) ≥ highest_var p_f - (n + 1) := by
+      suffices h : offset f_h g_h ≥ highest_var p_f from Nat.sub_le_sub_right h (n + 1)
+      simp [offset]
     have := cleanly_computable_append_zeros_append_xs f_h ([x] ++ xs) ⟨xs, xs_l⟩ this
     simp [init_state] at this
     simp
     rw [this]
 
-theorem execution_from_state_prec_program_1_4 (f_h : cleanly_computes p_f f) (g_h : cleanly_computes p_g g) (v : VectNat (n + 1)) :
-    execution_from_state (f v.tail :: v.tail.toList ++ 0 :: 0 :: List.zeros (offset f_h g_h - (n + 2)) ++ 0 :: v.toList) (X (offset f_h g_h + 1) += X 0)
-      = f v.tail :: v.tail.toList ++ 0 :: 0 :: List.zeros (offset f_h g_h - (n + 2)) ++ f v.tail :: v.toList := by
-  exact calc
-    execution_from_state (f v.tail :: v.tail.toList ++ 0 :: 0 :: List.zeros (offset f_h g_h - (n + 2)) ++ 0 :: v.toList) (X (offset f_h g_h + 1) += X 0)
-      =
-    execution_from_state ((f v.tail :: v.tail.toList ++ 0 :: 0 :: List.zeros (offset f_h g_h - (n + 2))) ++ 0 :: v.toList) (X (offset f_h g_h + 1) += X 0) := by simp
-    _ = f v.tail :: v.tail.toList ++ 0 :: 0 :: List.zeros (offset f_h g_h - (n + 2)) ++ f v.tail :: v.toList := by
-      have : (f v.tail :: v.tail.toList ++ 0 :: 0 :: List.zeros (offset f_h g_h - (n + 2))).length = offset f_h g_h + 1 := by
-        simp
-        rewrite [Nat.add_comm, Nat.add_assoc, Nat.add_assoc]
-        have : 1 + (1 + n) = n + 2 := by simp_arith
-        rewrite [this]
-        have : offset f_h g_h ≥ n + 2 := by dsimp [offset] ; exact Nat.le_max_left _ _
-        exact Nat.sub_add_cancel this
-      rewrite [inc_X_i_X_j_adds_value this]
-      simp [value_at]
-
-theorem execution_from_state_prec_program_1_5 (f_h : cleanly_computes p_f f) (g_h : cleanly_computes p_g g) (v : VectNat (n + 1)) :
-    execution_from_state (f v.tail :: v.tail.toList ++ 0 :: 0 :: List.zeros (offset f_h g_h - (n + 2)) ++ f v.tail :: v.toList) (CLEAR X 0)
-      = 0 :: v.tail.toList ++ 0 :: 0 :: List.zeros (offset f_h g_h - (n + 2)) ++ (f v.tail) :: v.toList := by
-  simp [execution_from_state, clear_value_cons_zero]
-
-theorem execution_from_state_prec_program_1 (f_h : cleanly_computes p_f f) (g_h : cleanly_computes p_g g) (v : VectNat (n + 1)) :
-    execution_from_state (0 :: v.toList ++ 0 :: List.zeros (offset f_h g_h - (n + 2)) ++ 0 :: 0 :: List.zeros n) (prec_program_1 f_h g_h)
-      = 0 :: v.tail.toList ++ 0 :: 0 :: List.zeros (offset f_h g_h - (n + 2)) ++ (f v.tail) :: v.toList := by
-  let p_1_1 := store_X_1_to_X_succ_n (offset f_h g_h + 2) n
+theorem execution_from_state_prec_program_1 (v : VectNat (n + 1)) :
+    execution_from_state (0 :: v.toList ++ 0 :: List.zeros (offset f_h g_h - (n + 2)) ++ 0 :: List.zeros n) (prec_program_1 f_h g_h)
+      = f v.tail :: v.tail.toList ++ 0 :: 0 :: List.zeros (offset f_h g_h - (n + 2)) ++ v.toList := by
+  let p_1_1 := store_X_1_to_X_succ_n (offset f_h g_h + 1) n
   let p_1_2 := clear_X_j_to_X_n_plus_j 1 n
   let p_1_3 := match n with
     | 0 => p_f
-    | n + 1 => setup_X_j_to_X_n_plus_j (offset f_h g_h + 2) 1 n ++ p_f
-  let p_1_4 := X (offset f_h g_h + 1) += X 0
-  let p_1_5 := CLEAR X 0
-  have : prec_program_1 f_h g_h = p_1_1 ++ p_1_2 ++ p_1_3 ++ p_1_4 ++ p_1_5 := by
-    dsimp [prec_program_1, p_1_1, p_1_2, p_1_3, p_1_4, p_1_5]
+    | n + 1 => setup_X_j_to_X_n_plus_j (offset f_h g_h + 1) 1 n ++ p_f
+  have : prec_program_1 f_h g_h = p_1_1 ++ p_1_2 ++ p_1_3:= by
+    dsimp [prec_program_1, p_1_1, p_1_2, p_1_3]
+
   rewrite [this]
   repeat rewrite [concat_is_seq_execution]
   simp [execution_from_state]
-  dsimp [p_1_1, p_1_2, p_1_3, p_1_4, p_1_5]
+  dsimp [p_1_1, p_1_2, p_1_3]
   rewrite [execution_from_state_prec_program_1_1, execution_from_state_prec_program_1_2,
-    execution_from_state_prec_program_1_3, execution_from_state_prec_program_1_4,
-    execution_from_state_prec_program_1_5]
+    execution_from_state_prec_program_1_3]
   simp
+
+-- 0 :: 0 :: 0 :: List.zeros n ++ List.zeros (offset f_h g_h - (n + 2)) ++ 0 :: (f v.tail) :: v.toList
+-- 0 :: k :: 0 :: List.zeros n ++ List.zeros (offset f_h g_h - (n + 2)) ++ 0 :: (f v.tail) :: v.toList
+-- theorem execution_from_state_prec_program_2_1 : 2 = 3 := by
+--   sorry
 
 -- TODO: check if clear is correct
 -- theorem execution_from_state_prec_program_2_1 (f_h : cleanly_computes p_f f) (g_h : cleanly_computes p_g g) (v : VectNat (n + 1)) :
